cedar-lean/Cedar/Thm/Validation/WellTyped/GetAttr.lean
@@ -1,0 +1,84 @@
+/-
+ Copyright Cedar Contributors
+
+ Licensed under the Apache License, Version 2.0 (the "License");
+ you may not use this file except in compliance with the License.
+ You may obtain a copy of the License at
+
+      https://www.apache.org/licenses/LICENSE-2.0
+
+ Unless required by applicable law or agreed to in writing, software
+ distributed under the License is distributed on an "AS IS" BASIS,
+ WITHOUT WARRANTIES OR CONDITIONS OF ANY KIND, either express or implied.
+ See the License for the specific language governing permissions and
+ limitations under the License.
+-/
+import Cedar.Validation.TypedExpr
+import Cedar.Thm.Validation.WellTyped.Definition
+import Cedar.Thm
+import Cedar.Spec
+
+namespace Cedar.Thm
+
+open Cedar.Validation
+open Cedar.Thm
+open Cedar.Spec
+
+theorem well_typed_is_sound_get_attr_entity
+{v : Value}
+{env : Environment}
+{request : Request}
+{entities : Entities}
+{ety : EntityType}
+{rty : RecordType}
+{x₁ : TypedExpr}
+{attr : Attr}
+{ty : CedarType}
+(h₁ : RequestAndEntitiesMatchEnvironment env request entities)
+(h₂ : WellTypedIsSound x₁)
+(h₃ : TypedExpr.WellTyped env x₁)
+(h₄ : x₁.typeOf = CedarType.entity ety)
+(h₅ : env.ets.attrs? ety = some rty)
+(h₆ : Option.map Qualified.getType (Data.Map.find? rty attr) = some ty)
+(h₇ : (do
+  let v₁ ← evaluate x₁.toExpr request entities
+  getAttr v₁ attr entities) = Except.ok v) :
+InstanceOfType v (x₁.getAttr attr ty).typeOf
+:= by
+  simp only [WellTypedIsSound] at h₂
+  generalize hᵢ' : evaluate x₁.toExpr request entities = res₁
+  cases res₁ <;> simp [hᵢ'] at h₇
+  replace h₂ := h₂ h₁ h₃ hᵢ'
+  simp only [h₄] at h₂
+  cases h₂
+  rename_i het
+  simp only [InstanceOfEntityType] at het
+  simp only [RequestAndEntitiesMatchEnvironment, InstanceOfEntitySchema] at h₁
+  rcases h₁ with ⟨_, h₁, _⟩
+  simp [getAttr, attrsOf, Entities.attrs, Data.Map.findOrErr] at h₇
+  rename_i uid _ _
+  split at h₇
+  · simp only [Except.bind_ok] at h₇
+    rename_i data heq
+    have ⟨entry, h₁₁, _, h₁₂, _⟩  := h₁ uid data heq
+    split at h₇
+    · rename_i v₁ heq₁
+      simp only [Except.ok.injEq] at h₇
+      cases h₁₂
+      rename_i h₈ _
+      simp only [EntitySchema.attrs?, Option.map_eq_some'] at h₅
+      rcases h₅ with ⟨a, h₅₁, h₅₂⟩
+      simp [←het] at h₁₁
+      simp only [h₁₁, Option.some.injEq] at h₅₁
+      simp only [← h₅₁] at h₅₂
+      have h₈ := λ qty => h₈ attr v₁ qty heq₁
+      simp only [h₅₂] at h₈
+      simp only [Option.map_eq_some'] at h₆
+      rcases h₆ with ⟨qty, h₆₁, h₆₂⟩
+      have h₈ := h₈ qty h₆₁
+      simp only [h₆₂] at h₈
+      simp [TypedExpr.typeOf, ←h₇]
+      exact h₈
+    · cases h₇
+  · simp only [Except.bind_err, reduceCtorEq] at h₇
+end Cedar.Thm
